List images for partial functions.
To define partial functions I now use a list of appropriate size (given by a dependent type family) as the range of functions rather than a list of pair. Makes it possible to reuse the notion of finite set more directly. The proofs are significantly simpler, and can be split into smaller units of meaning.

This follows a suggestion by Cyril Cohen.

FinMap.v
@@ -14,8 +14,15 @@ Require Import FinSet.Quotients.Retract.
 Require Import FinSet.Quotients.Countable.
 Require Import FinSet.FinSet.
 Import FinSet.Notations.
+Require FinSet.Lib.Image.
 
 Module CofinitelyConstant.
+
+ (** The definition of functions as a pair of a [FinSet.T] and a
+     dependently typed list of corresponding size has been suggested
+     by Cyril Cohen. *)
+
+ Import Image.Coercions.
 
  (** Decidably distinguished point in a type. *)
  Record Distinguished (A:Type) := {
@@ -29,196 +36,108 @@ Module CofinitelyConstant.
    dec := Sumbool.sumbool_not _ _ (x.(distinguished) y)
  |}.
 
- Program  Definition T A {_:Countable A} (B:Type) (x:Distinguished B) :=
-   { l:list (A*B) | Canonize (
-                      eq_countable
-                        (List.map fst l) 
-                        (listset.(inj) (listset.(proj) (List.map fst l)))
-                   && ListSet.dforall
-                        (Distinct_from x)
-                        (List.map snd l)
-   )}.
-
- Fixpoint assoc {A} {c:Countable A} {B} (d:B) (x:A) (l:list (A*B)) : B :=
-   match l with
-   | nil => d
-   | cons (a,b) q => if dec (eq_countable x a) then b else assoc d x q
-   end
- .
+ Record T A {C:Countable A} (B:Type) (x:Distinguished B) := {
+   support : FinSet.T A ;
+   range   : Image.T B (listset.(inj) support) ;
+   reduced : Canonize (ListSet.dforall (Distinct_from x) range)
+ }.
+ Arguments range {A C B x} _.
+ Arguments support {A C B x} _.
 
  Definition fun_of {A} {_:Countable A} {B x} (f:T A B x) (a:A) : B :=
-   assoc x.(pt) a (proj1_sig f).
+   Image.assoc eq_countable x.(pt) f.(range) a.
 
  Coercion fun_of : T >-> Funclass.
+
+ Lemma support_spec A (_:Countable A) B x (f:T A B x) :
+   forall a:A, a∈(support f) <-> f a <> x.(pt).
+ Proof.
+   intros a. destruct f as [s img reduced_img]. cbn. unfold mem.
+     rewrite canonize_spec in reduced_img. revert img reduced_img.
+     generalize (listset.(inj) s). clear s. intros l img reduced_img.
+   induction l as [ | a' l hl ].
+   + split.
+     * intros. ListSet.use_no_mem_list_empty.
+     * refine match img with Image.inil => _ end. cbn.
+       congruence.
+   + revert reduced_img hl.
+     refine match img with Image.icons b img' => _ end. cbn [Image.assoc].
+       intros reduced_img hl.
+     destruct dec as [ha'|ha']. all:cbn in ha'.
+     * subst a. clear hl. cbn in reduced_img |- *.
+       split.
+       - now specialize (reduced_img (ListSet.head b)).
+       - intros _.
+         now exists (ListSet.head _).
+     * rewrite <- hl; cycle 1.
+       { cbn in reduced_img |-*. intros m.
+         now specialize (reduced_img (ListSet.tail m)). }
+       split.
+       - cbn. intros [m hm]. revert ha' hm.
+         refine match m with ListSet.head a => _ | ListSet.tail m' => _ end.
+         { cbn. congruence. }
+         intros _ hm. cbn in hm.
+         now exists m'.
+       - cbn. intros [m hm].
+         now exists (ListSet.tail m).
+ Qed.
 
  Lemma ext A (_:Countable A) B x :
    forall f g:T A B x, (forall a, f a = g a) -> f = g.
  Proof.
-   assert (forall (l:list (A*B)) (a:A),
-     ListSet.dforall (Distinct_from x) (List.map snd l) ->
-     Distinct_from x (assoc x.(pt) a l) ->
-     ListSet.mem_list eq_countable a (List.map fst l))
-   as mem_domain.
-   { cbn. intros l.
-     induction l as [ | [a₀ b₀] l hl ].
-     + cbn. congruence.
-     + cbn -[eq_countable]. intros a h₂ hass.
-       destruct dec as [ha|ha].
-       * exists (ListSet.head _).
-         now cbn in ha|-*.
-       * apply hl in hass; cycle 1.
-         { refine (fun m => h₂ (ListSet.tail m)). }
-         destruct hass as [m hm].
-         exists (ListSet.tail m). cbn.
-         trivial. }
-   assert (forall (l:list (A*B)) (m₁:ListSet.Mem (List.map fst l)),
-           exists (m₂:ListSet.Mem (List.map snd l)),
-             ListSet.of_mem m₂ = assoc x.(pt) (ListSet.of_mem m₁) l)
-   as assoc_mem.
-   { fix assoc_mem 2. intros l m.
-     destruct l as [|[a b] l].
-     { cbn in m. ListSet.use_no_mem_empty. }
-     cbn  -[eq_countable] in m|-*.
-     destruct dec as [ha|ha].
-     + now exists (ListSet.head _).
-     + revert ha.
-       refine (match m in ListSet.Mem l' return l' = cons a (List.map fst l) -> _ with | ListSet.head a' => _ | ListSet.tail m' => _ end eq_refl).
-       { cbn. congruence. }
-       intros [= _ ->] _.
-       specialize (assoc_mem _ m').
-       destruct assoc_mem as [m'' hm''].
-       now exists (ListSet.tail m'').
-     Guarded. }
-   assert (forall l₁ l₂:list(A*B),
-     ListSet.dforall (Distinct_from x) (List.map snd l₁) ->
-     (forall a, assoc x.(pt) a l₁ = assoc x.(pt) a l₂) ->
-     ListSet.included_list eq_countable (List.map fst l₁) (List.map fst l₂))
-   as incl_domain.
-   { intros l₁ l₂ nx₁ h. cbn. intros m₁.
-     destruct (dec (Distinct_from x (assoc x.(pt) (ListSet.of_mem m₁) l₁)))
-       as [hm|hm]; cycle 1.
-     { cbn in hm,nx₁.
-       specialize (assoc_mem _ m₁).
-       destruct assoc_mem as [m₁' hm₁].
-       rewrite <- hm₁ in *.
-       congruence. }
-     rewrite h in hm. cbn in hm.
-     revert hm. generalize (ListSet.of_mem m₁). clear l₁ nx₁ h m₁.
-     induction l₂ as [|[a b] l hl].
-     { cbn. congruence. }
-     cbn -[eq_countable]. intros a' h.
-     destruct dec as [->|ha].
-     + now exists (ListSet.head _).
-     + apply hl in h. destruct h as [m hm].
-       now exists (ListSet.tail m). }
-   assert (forall (a:A) (l:list (A*B)),
-             Denies (ListSet.mem_list eq_countable a (List.map fst l)) ->
-             assoc x.(pt) a l = x.(pt))
-   as denies_assoc.
-   { intros a l. induction l as [|[a' b'] l hl].
-     + trivial.
-     + cbn -[eq_countable]. intros h.
-       destruct dec as [c|_].
-       { specialize (h (ListSet.head _)).
-         cbn in *. contradiction. }
-       apply hl. cbn in *.
-       intros m. specialize (h (ListSet.tail m)).
-       exact h. }
-   assert (forall l₁ l₂:list(A*B),
-     ListSet.dforall (Distinct_from x) (List.map snd l₁) ->
-     ListSet.dforall (Distinct_from x) (List.map snd l₂) ->
-     (forall a, assoc x.(pt) a l₁ = assoc x.(pt) a l₂) ->
-     ListSet.eq_set_list eq_countable (List.map fst l₁) (List.map fst l₂))
-   as eq_domain.
-   { intros **. split.
-     all: now apply incl_domain. }
-   assert (forall l₁ l₂:list (A*B),
-             ListSet.nodup eq_countable (List.map fst l₁) ->
-             ListSet.nodup eq_countable (List.map fst l₂) ->
-             ListSet.dforall (Distinct_from x) (List.map snd l₁) ->
-             ListSet.dforall (Distinct_from x) (List.map snd l₂) ->
-             List.map fst l₁ = List.map fst l₂ ->
-             (forall a, assoc x.(pt) a l₁ = assoc x.(pt) a l₂) ->
-             l₁=l₂)
-   as assoc_ext.
-   { intros l₁. induction l₁ as [|[a₁ b₁] l₁ hl₁].
-     + intros [|[a₂ b₂] l₂];cycle 1.
-       { cbn. congruence. }
-       trivial.
-     + intros [|[a₂ b₂] l₂].
-       { cbn. congruence. }
-       cbn -[eq_countable]. intros [h₁ h₂] [h₃ h₄] h₅ h₆ [= <- h₇] h₈.
-       f_equal.
-       { f_equal.
-         specialize (h₈ a₁).
-         destruct dec as [_|n];cycle 1.
-         { cbn in n. congruence. }
-         congruence. }
-       apply hl₁.
-       * assumption.
-       * assumption.
-       * intros m. specialize (h₅ (ListSet.tail m)).
-         trivial.
-       * intros m. specialize (h₆ (ListSet.tail m)).
-         trivial.
-       * assumption.
-       * intros a. specialize (h₈ a).
-         destruct dec as [<-|_].
-         { rewrite !denies_assoc.
-           { trivial. }
-           all:assumption. }
-         trivial. }
-   (* /intermediate lemmas *)
-   (* rearranging goal *)
-   intros [f hf] [g hg] h. cbn in h.
-   apply dsigma_ext. cbn. rewrite !canonize_spec in hf,hg.
-   cbn -[inj proj] in hf,hg.
-   destruct hf as [hf₁ hf₂], hg as [hg₁ hg₂].
-   (* /rearranging goal *)
-   apply assoc_ext.
-   all: try solve[try rewrite hf₁;try rewrite hg₁; auto using set_nodup].
-   rewrite hf₁,hg₁. f_equal.
-   apply set_ext. unfold mem.
-   rewrite <-hf₁, <-hg₁. intros a.
-   apply ListSet.mem_eq_set_list.
-   { typeclasses eauto. }
-   apply eq_domain.
-   all:eauto.
- Qed.
-
- Definition support {A} {_:Countable A} {B x} (f:T A B x) : FinSet.T A :=
-   listset.(proj) (List.map fst (proj1_sig f)).
-
- Lemma mem_support A B x (_:Countable A) : forall f:T A B x,
-   forall y, y∈(support f) <-> f y<>x.(pt).
- Proof.
-   intros [f hf] y. unfold support. unfold fun_of. cbn [proj1_sig].
-   rewrite canonize_spec in hf. destruct hf as [hf₁ hf₂].
-   unfold FinSet.mem. rewrite <- hf₁. clear hf₁.
-   induction f as [|[a b] l hl].
-   + cbn. split.
-     * intros [m _]. ListSet.use_no_mem_empty.
-     * congruence.
-   + cbn -[eq_countable]. destruct dec as [ha|ha].
-     * cbn in hf₂. specialize (hf₂ (ListSet.head b)). cbn in hf₂.
-       split.
-       - trivial.
-       - intros _. exists (ListSet.head a).
-         trivial.
-     * rewrite <- hl; cycle 1.
-       { cbn in hf₂|-*. intros m.
-         now specialize (hf₂ (ListSet.tail m)). }
-       split.
-       - intros [m hm]. revert ha hm.
-         refine match m with
-                | ListSet.head a' => _
-                | ListSet.tail m' => _
-                end.
-         { cbn. congruence. }
-         cbn. intros _ h.
-         eexists. eauto.
-       - intros [m hm].
-         now exists (ListSet.tail m).
+   assert (forall f g : T A B x, (forall a, f a = g a) -> support f ⊆ support g)
+      as incl_support.
+   { unfold subset. intros f g h a ha. cbn.
+     rewrite support_spec in *. congruence. }
+   assert (forall f g : T A B x, (forall a, f a = g a) -> support f = support g)
+      as eq_support.
+   { intros **.
+     apply double_inclusion.
+     all:eauto. }
+   assert (forall (l:list A) (f g:Image.T B l),
+               ListSet.nodup eq_countable l ->
+               ListSet.dforall (Distinct_from x) f ->
+               ListSet.dforall (Distinct_from x) g ->
+               (forall a, Image.assoc eq_countable x.(pt) f a = Image.assoc eq_countable x.(pt) g a) ->
+               f=g) as eq_range.
+   { intros * hl hf hg h.
+     induction l as [|a l ihl].
+     { refine match f with Image.inil => _ end.
+       refine match g with Image.inil => _ end.
+       reflexivity. }
+     revert g hl hf hg h ihl.
+     refine match f with Image.icons b q => _ end. clear. intros g.
+     revert b q.
+     refine match g with Image.icons b' q' => _ end. clear.
+     intros b q hl hf hg h ihl.
+     rewrite ihl with (f:=q) (g:=q').
+     { apply Image.ext. cbn. f_equal.
+       specialize (h a). (* spiwack: I think 'a' is a generated name here *)
+       unfold Image.assoc in h. destruct dec as [_|c];cycle 1.
+       { clear -c. cbn in c. congruence. }
+       assumption. }
+     + clear -hl. cbn in *. tauto.
+     + clear -hf. cbn in *.
+       intros m. specialize (hf (ListSet.tail m)). cbn in hf.
+       assumption.
+     + clear -hg. cbn in *.
+       intros m. specialize (hg (ListSet.tail m)). cbn in hg.
+       assumption.
+     + clear -h hl. intros a'. specialize (h a'). cbn [Image.assoc] in h.
+       destruct dec as [<-|h'].
+       { cbn in hl. transitivity (x.(pt)).
+         all: rewrite Image.assoc_default;[reflexivity|]. all:cbn.
+         all: destruct hl as [_ hl]. all:solve[firstorder]. }
+       assumption. }
+   intros f g h. specialize (eq_support f g h).
+   destruct f as [sf rf rdf], g as [sg rg rdg]. cbn -[ListSet.dforall] in *. destruct eq_support.
+   apply eq_range in h;cycle 1.
+   { apply set_nodup. }
+   { now rewrite canonize_spec in *. }
+   { now rewrite canonize_spec in *. }
+   destruct h.
+   f_equal.
+   apply irrelevant_canonize.
  Qed.
 
 End CofinitelyConstant.
@@ -249,9 +168,9 @@ Module Partial.
  Definition domain {A} {_:Countable A} {B} (f:T A B) : FinSet.T A :=
    CofinitelyConstant.support f.
 
- Lemma mem_domain A B (_:Countable A) : forall f:T A B,
+ Lemma domain_spec A B (_:Countable A) : forall f:T A B,
    forall y, y∈(domain f) <-> f y<>None.
- Proof. apply CofinitelyConstant.mem_support. Qed.
+ Proof. apply CofinitelyConstant.support_spec. Qed.
 
 End Partial.
 
@@ -278,7 +197,7 @@ Module CofinitelyId.
    apply dsigma_ext. cbn. unfold fun_of in *. cbn [proj1_sig] in *.
    rewrite !canonize_spec in *. cbn -[Partial.domain] in hf,hg.
    apply Partial.ext. intros a. specialize (h a).
-   specialize (hf a). specialize (hg a). rewrite Partial.mem_domain in hf,hg.
+   specialize (hf a). specialize (hg a). rewrite Partial.domain_spec in hf,hg.
    destruct Partial.fun_of,Partial.fun_of.
    all: try congruence.
    + destruct hf; congruence.
@@ -288,16 +207,16 @@ Module CofinitelyId.
  Definition support {A} {_:Countable A} (f:T A) : FinSet.T A :=
    Partial.domain (proj1_sig f).
 
- Lemma mem_support A (_:Countable A) : forall f:T A,
+ Lemma support_spec A (_:Countable A) : forall f:T A,
    forall y, y∈(support f) <-> f y<>y.
  Proof.
    intros [f hf] y. unfold support,fun_of. cbn -[Partial.domain].
    rewrite canonize_spec in hf. cbn -[Partial.domain] in hf.
    specialize (hf y).
    split.
-   + intros hy. specialize (hf hy). rewrite Partial.mem_domain in hy.
+   + intros hy. specialize (hf hy). rewrite Partial.domain_spec in hy.
      destruct Partial.fun_of. all:congruence.
-   + rewrite Partial.mem_domain.
+   + rewrite Partial.domain_spec.
      destruct Partial.fun_of. all:congruence.
  Qed.
 
