Lib/Image.v
@@ -1,0 +1,134 @@
+(** List with the same size of another list. This constitutes the
+    prototype of finite functions. This module is inspired by the
+    [ffun] module in Ssreflect. Ssreflect's [ffun] is somehow smarter
+    though, as it restricts its attention to lists without duplicate
+    in a type with decidable equality, so that there are stronger
+    extensionality principles. *)
+
+Require Import Coq.Classes.RelationClasses.
+Require Import Coq.Lists.List.
+Import ListNotations.
+Require Import FinSet.Lib.DProp.
+Require FinSet.Lib.ListSet.
+
+Inductive T {A B:Type} : list A -> Type :=
+| inil : T []
+| icons {a l} (b:B) (q:T l) : T (a::l)
+.
+Arguments T {A} B l : clear implicits.
+
+Fixpoint to_list {A B} {l:list A} (q:T B l) : list B :=
+  match q with
+  | inil => []
+  | icons b q => b::(to_list q)
+  end
+.
+
+Lemma ext A B (l:list A) :
+  forall q₁ q₂:T B l, to_list q₁ = to_list q₂ -> q₁ = q₂.
+Proof.
+  intros q₁. induction q₁ as [ ? ? | ? ?  b₁ q₁ hq₁].
+  + intros q₂. refine match q₂ with inil => _ end.
+    reflexivity.
+  + intro q₂. revert b₁ q₁ hq₁.
+    refine match q₂ with icons b₂ q₂ => _ end. intros b₁ q₁ hq₁. cbn.
+    intros [= <- h]. f_equal.
+    eauto.
+Qed.
+
+
+(** [Image.T] can be read as an association list with the domain as
+    keys. In this variant we return a default value when there is no
+    corresponding key. *)
+Fixpoint assoc {A B} {l:list A} (E:A->A->DProp) (d:B) (q:T B l) (x:A) : B :=
+  match l return T B l -> B with
+  | [] => fun _ => d
+  | a::l => fun q =>
+    match q with icons b q =>
+      if dec (E x a) then b
+      else assoc E d q x
+    end
+  end q
+.
+
+Lemma assoc_default A B (l:list A) E d (q:T B l) : forall x, ~(ListSet.mem_list E x l) -> assoc E d q x = d.
+Proof.
+  intros x.
+  induction l as [|a l hl].
+  + refine match q with inil => _ end. cbn.
+    reflexivity.
+  + revert hl.
+    refine match q with icons b q' => _ end. cbn [assoc].
+    intros hl h.
+    destruct dec as [hx|_].
+    { cbn in h. contradiction h.
+      now eexists (ListSet.head _). }
+    apply hl. cbn in h|-*.
+    intros [m hm]. apply h.
+    now exists (ListSet.tail m).
+Qed.
+
+(** Conversely, given a function defined on a domain we can create the
+    image of the domain. *)
+Fixpoint img {A B} (l:list A) : (ListSet.Mem l -> B) -> T B l :=
+  match l with
+  | [] => fun _ => inil
+  | a::l => fun f =>
+    icons (f (ListSet.head a)) (img l (fun m => f (ListSet.tail m)))
+  end
+.
+
+(** Variant of [img] with decidable equality *)
+Program Definition img_dec {A B} (E:A->A->DProp) {_:Reflexive E} (l:list A) (f:forall x:A, Canonize (ListSet.mem_list E x l) -> B) : T B l :=
+  img l (fun m => f (ListSet.of_mem m) _).
+Next Obligation.
+  intros **. apply canonize_spec.
+  eexists. reflexivity.
+Qed.
+
+Lemma assoc_img₀ A B (E:A->A->DProp) (_:Reflexive E)
+      (d:B) l m f :
+  (forall u v, E u v -> u=v) ->
+  (forall m m':ListSet.Mem l, ListSet.of_mem m = ListSet.of_mem m' -> f m = f m') ->
+  assoc E d (img l f) (ListSet.of_mem m) = f m.
+Proof.
+  intros e_eq f_ext.
+  induction l as [ | a l hl ].
+  { ListSet.use_no_mem_empty. }
+  cbn. destruct dec as [he|he].
+  + apply e_eq in he.
+    now apply f_ext.
+  + revert he f f_ext hl.
+    refine match m with ListSet.head a' => _ | ListSet.tail m' => _ end.
+    { intros he f _ _. cbn in he. rewrite denies_spec in he.
+      now pose proof (reflexivity a') as he'. }
+    intros _ f f_ext hl. cbn.
+    apply hl.
+    eauto.
+Qed.
+
+Lemma assoc_img A B (E:A->A->DProp) (_:Reflexive E)
+      (d:B) l x (h:Canonize (ListSet.mem_list E x l)) f :
+  (forall u v, E u v -> u=v) -> assoc E d (img_dec E l f) x = f x h.
+Proof.
+  intros e_eq.
+  assert (forall y hy z hz, y=z -> f y hy = f z hz) as f_ext.
+  { intros y hy z hz <-. f_equal.
+    apply irrelevant_canonize. }
+  unfold img_dec.
+  pose proof h as h'. apply canonize_spec in h'.
+  pose proof (ListSet.mem_of_mem_list_spec _ _ _ _ h') as hx.
+  apply e_eq in hx. rewrite hx at 1.
+  rewrite assoc_img₀;cycle 1.
+  { typeclasses eauto. }
+  { assumption. }
+  { intros **.
+    now apply f_ext. }
+  now apply f_ext.
+Qed.
+
+Module Coercions.
+
+  Coercion to_list : T >-> list.
+
+End Coercions.
